reorganise files

basicReflectionLib.sml
@@ -1,0 +1,112 @@
+structure basicReflectionLib = struct
+local
+  open HolKernel boolLib bossLib holSyntaxSyntax listSyntax pairSyntax stringSyntax
+in
+
+fun n_imp_and_intro 0 = ALL_CONV
+  | n_imp_and_intro n = REWR_CONV (GSYM AND_IMP_INTRO) THENC
+                       (RAND_CONV (n_imp_and_intro (n-1)))
+
+datatype type_view = Tyvar of string | Tyapp of string * string * hol_type list
+
+local open String in
+fun tyvar_to_deep s =
+  if sub(s,0) = #"'" then
+    if size s = 2 then str(Char.toUpper (sub(s,1)))
+    else extract(s,1,NONE)
+  else s
+end
+
+fun type_view (ty : hol_type) =
+  if is_type ty then
+    case dest_thy_type ty of { Args = args, Thy = thy, Tyop = tyop } =>
+      Tyapp (thy, tyop, args)
+  else
+    Tyvar (tyvar_to_deep (dest_vartype ty))
+
+fun type_to_deep ty = case type_view ty of
+    Tyvar name => mk_Tyvar (fromMLstring name)
+  | Tyapp (thy,name,args) =>
+      mk_Tyapp(fromMLstring name, mk_list(List.map type_to_deep args, type_ty))
+
+fun term_to_deep tm =
+  case dest_term tm of
+    VAR(x,ty) => mk_Var(fromMLstring x, type_to_deep ty)
+  | CONST {Name,Thy,Ty} => mk_Const(fromMLstring Name, type_to_deep Ty)
+  | COMB (f,x) => mk_Comb(term_to_deep f, term_to_deep x)
+  | LAMB (x,b) =>
+      let
+        val (x,ty) = dest_var x
+      in
+        mk_Abs(fromMLstring x, type_to_deep ty, term_to_deep b)
+      end
+
+fun underscores [] = ""
+  | underscores (x::xs) = "_" ^ x ^ underscores xs
+
+fun type_name (ty : hol_type) = case type_view ty of
+    Tyvar name            => tyvar_to_deep name
+  | Tyapp (thy,tyop,args) => tyop ^ underscores (map type_name args)
+
+val U = mk_vartype("'U")
+fun mk_in_var (ty : hol_type) =
+  mk_var ("in_" ^ type_name ty, ty --> U)
+
+val mem = ``mem:'U->'U->bool``
+local
+  open holSemanticsTheory
+  fun genv x = (* genvar (type_of x) *)
+    variant [] x
+in
+  val tysig = genv ``tysig:tyenv``
+  val tmsig = genv ``tmsig:tmenv``
+  val tyass = genv ``tyass:'U tyass``
+  val tmass = genv ``tmass:'U tmass``
+  val tyval = genv ``tyval:'U tyval``
+  val tmval = genv ``tmval:'U tmval``
+end
+
+val signatur = mk_pair(tysig,tmsig)
+val interpretation = mk_pair(tyass,tmass)
+val valuation = mk_pair(tyval,tmval)
+val termsem_tm = ``termsem0 ^mem``
+fun mk_termsem d =
+  list_mk_comb(termsem_tm,[tmsig,interpretation,valuation,d])
+
+val EVAL_STRING_SORT =
+  CONV_TAC (DEPTH_CONV (fn tm => if can (match_term ``STRING_SORT (tyvars X)``) tm
+                        then EVAL tm else raise UNCHANGED))
+
+(* given [...,A,...] |- P and H |- A <=> B1 /\ ... /\ Bn
+   produce [...,B1,...,Bn,...] ∪ H |- P *)
+fun simplify_assum th simpth =
+  let
+    val A = lhs(concl simpth)
+    val th1 = DISCH A th
+    val th2 = CONV_RULE(LAND_CONV(REWR_CONV simpth)) th1
+    val n = length(strip_conj(rhs(concl simpth)))
+    val th3 = CONV_RULE (n_imp_and_intro (n-1)) th2
+  in
+    funpow n UNDISCH th3
+  end
+
+(* given [...,A',...] |- P and H |- !x1..xn. B1 /\ ... /\ Bn ==> A
+   produce [...,B1',...,Bn',...] ∪ H |- P *)
+fun replace_assum th simpth =
+  let
+    val c = simpth |> concl
+    val (xs,b) = c |> strip_forall
+    val (B,A) = dest_imp b handle HOL_ERR _ => (T,b)
+    val A' = first (can (match_term A)) (hyp th)
+    val th1 = DISCH A' th
+    val (s,_) = match_term A A'
+    val th2 = ISPECL (map (fn x => #residue(first (equal (fst(dest_var x)) o fst o dest_var o #redex) s)) xs) simpth
+    val n = B |> strip_conj |> length
+    val th3 = CONV_RULE (n_imp_and_intro (n-1)) th2
+    val th4 = funpow n UNDISCH th3 handle HOL_ERR _ => th3
+  in
+    MP th1 th4
+  end
+
+end
+end
