reflectionScript.sml
@@ -1,13 +1,12 @@
 open HolKernel boolLib bossLib lcsymtacs
-open miscLib pred_setTheory setSpecTheory holSemanticsTheory
+open miscLib basicReflectionLib pred_setTheory
+open setSpecTheory holSyntaxTheory holSemanticsTheory holSemanticsExtraTheory
 
 val _ = temp_tight_equality()
 val _ = new_theory"reflection"
 
 val finv_def = Define`
   finv f x = @y. f y = x`
-
-val mem = ``mem:'U->'U->bool``
 
 val is_in_def = xDefine"is_in"`
   is_in0 ^mem f = ∃x. BIJ f UNIV {a | mem a x}`
@@ -166,7 +165,7 @@ val range_in_fun = store_thm("range_in_fun",
   match_mp_tac (UNDISCH abstract_eq) >> simp[] >>
   metis_tac[is_in_finv_right,is_in_finv_left])
 
-val finv_in_bool_True = store_thm("finv_in_bool_True",
+val finv_in_bool_True = prove(
   ``is_set_theory ^mem ⇒ finv in_bool True``,
   rw[] >>
   imp_res_tac is_in_in_bool >>
@@ -175,8 +174,9 @@ val finv_in_bool_True = store_thm("finv_in_bool_True",
   metis_tac[is_in_finv_left])
 
 val provable_imp_eq_true = store_thm("provable_imp_eq_true",
-  ``is_set_theory ^mem ∧
-    i models thy ∧
+  ``∀thy i v.
+    is_set_theory ^mem ⇒
+    i models thy ⇒
     is_valuation (tysof (sigof thy)) (tyaof i) v
     ⇒
     ∀p. (thy,[]) |- p ⇒ termsem (tmsof (sigof thy)) i v p = True``,
@@ -184,5 +184,160 @@ val provable_imp_eq_true = store_thm("provable_imp_eq_true",
   imp_res_tac holSoundnessTheory.proves_sound >>
   fs[entails_def] >> res_tac >>
   fs[satisfies_def])
+
+val mp_lemma = store_thm("mp_lemma",
+  ``(a ==> b) /\ (c ==> a) ==> (c ==> b)``,
+  metis_tac[])
+
+val good_context_def = Define`
+  good_context ^mem ^tysig ^tmsig ^tyass ^tmass ^tyval ^tmval ⇔
+    is_set_theory ^mem ∧
+    is_std_sig ^signatur ∧
+    is_interpretation ^signatur ^interpretation ∧
+    is_std_interpretation ^interpretation ∧
+    is_valuation ^tysig ^tyass ^valuation`
+val good_context = good_context_def |> concl |> strip_forall |> snd |> lhs
+
+val finv_in_bool_True = prove(
+``^good_context ⇒
+  (finv in_bool x ⇒ y) ⇒ ((x = True) ⇒ y)``,
+  metis_tac[finv_in_bool_True,good_context_def]) |> UNDISCH
+
+val _ = save_thm("finv_in_bool_True",finv_in_bool_True)
+
+val Var_thm = prove(
+  ``^tmval (x,ty) = inty v ⇒
+    ∀mem. inty v = termsem0 mem ^tmsig ^interpretation ^valuation (Var x ty)``,
+  rw[termsem_def])
+
+val Const_thm = prove(
+  ``instance ^tmsig ^interpretation name ty ^tyval = inty c ⇒
+    ∀mem. inty c = termsem0 mem ^tmsig ^interpretation ^valuation (Const name ty)``,
+  rw[termsem_def])
+
+val Comb_thm = prove(
+  ``^good_context ⇒
+    in_fun ina inb f = termsem ^tmsig ^interpretation ^valuation ftm ∧
+    ina x = termsem ^tmsig ^interpretation ^valuation xtm ⇒
+    is_in ina ⇒ is_in inb
+    ⇒
+    inb (f x) =
+      termsem ^tmsig ^interpretation ^valuation (Comb ftm xtm)``,
+  rw[good_context_def,termsem_def] >>
+  rpt(first_x_assum(SUBST1_TAC o SYM)) >>
+  rw[in_fun_def] >>
+  match_mp_tac EQ_SYM >>
+  match_mp_tac apply_abstract_matchable >>
+  simp[] >>
+  rw[is_in_range_thm] >>
+  AP_TERM_TAC >>
+  AP_TERM_TAC >>
+  match_mp_tac is_in_finv_left >>
+  simp[]) |> UNDISCH
+
+val Abs_thm = prove(
+  ``^good_context ⇒
+    ∀ina inb f x ty b.
+    range ina = typesem tyass tyval ty ⇒
+    range inb = typesem tyass tyval (typeof b) ⇒
+    is_in ina ⇒ is_in inb ⇒
+    (∀m. m <: range ina ⇒
+      inb (f (finv ina m)) =
+        termsem tmsig (tyass,tmass) (tyval,((x,ty) =+ m) tmval) b) ⇒
+    term_ok (tysig,tmsig) b
+    ⇒
+    in_fun ina inb f =
+      termsem tmsig (tyass,tmass) (tyval,tmval) (Abs x ty b)``,
+  rw[termsem_def,in_fun_def,good_context_def] >>
+  match_mp_tac (UNDISCH abstract_eq) >> simp[] >>
+  rw[] >>
+  match_mp_tac (UNDISCH termsem_typesem) >>
+  simp[] >>
+  qexists_tac`(tysig,tmsig)` >> simp[] >>
+  fs[is_std_interpretation_def] >>
+  fs[is_valuation_def,is_term_valuation_def] >>
+  simp[combinTheory.APPLY_UPDATE_THM] >>
+  rw[] >> metis_tac[]) |> UNDISCH
+
+val save_thms = map2 (curry save_thm)
+val _ = save_thms ["Var_thm","Const_thm","Comb_thm","Abs_thm"]
+                  [ Var_thm , Const_thm , Comb_thm , Abs_thm ]
+
+val good_context_is_in_in_bool = prove(mk_imp(good_context,rand(concl(is_in_in_bool))),
+  rw[good_context_def,is_in_in_bool]) |> UNDISCH
+
+val good_context_is_in_in_fun = prove(mk_imp(good_context,rand(concl(is_in_in_fun))),
+  rw[good_context_def,is_in_in_fun]) |> UNDISCH
+
+val good_context_lookup_bool = prove(
+  ``^good_context ⇒ FLOOKUP ^tysig "bool" = SOME 0``,
+  rw[good_context_def,is_std_sig_def]) |> UNDISCH
+
+val good_context_lookup_fun = prove(
+  ``^good_context ⇒ FLOOKUP ^tysig "fun" = SOME 2``,
+  rw[good_context_def,is_std_sig_def]) |> UNDISCH
+
+val good_context_extend_tmval = prove(
+  ``^good_context ∧
+     m <: typesem ^tyass ^tyval ty ⇒
+     good_context ^mem ^tysig ^tmsig ^tyass ^tmass ^tyval (((x,ty) =+ m) ^tmval)``,
+  rw[good_context_def,is_valuation_def,is_term_valuation_def,combinTheory.APPLY_UPDATE_THM] >>
+  rw[] >> rw[])
+
+val good_context_instance_equality = prove(
+  ``∀ty ina.
+    ^good_context ∧
+    type_ok ^tysig ty ∧
+    typesem ^tyass ^tyval ty = range ina ∧
+    is_in ina ⇒
+    instance ^tmsig ^interpretation "=" (Fun ty (Fun ty Bool)) ^tyval =
+      in_fun ina (in_fun ina in_bool) $=``,
+  rw[good_context_def] >>
+  fs[is_std_sig_def] >>
+  imp_res_tac instance_def >>
+  first_x_assum(qspec_then`[ty,Tyvar "A"]`mp_tac) >>
+  simp[holSyntaxLibTheory.REV_ASSOCD] >>
+  disch_then(mp_tac o SPEC interpretation) >>
+  simp[] >> disch_then kall_tac >>
+  EVAL_STRING_SORT >> simp[holSyntaxLibTheory.REV_ASSOCD] >>
+  fs[is_std_interpretation_def,interprets_def] >>
+  first_x_assum(qspec_then`("A"=+ typesem ^tyass ^tyval ty)(K boolset)`mp_tac) >>
+  discharge_hyps >- (
+    simp[is_type_valuation_def,combinTheory.APPLY_UPDATE_THM] >>
+    reverse(rw[mem_boolset]) >- metis_tac[] >>
+    qpat_assum`X = Y` (SUBST1_TAC o SYM) >>
+    match_mp_tac (UNDISCH typesem_inhabited) >>
+    fs[is_valuation_def,is_interpretation_def] >>
+    metis_tac[] ) >>
+  simp[combinTheory.APPLY_UPDATE_THM] >>
+  disch_then kall_tac >>
+  simp[in_fun_def] >>
+  match_mp_tac (UNDISCH abstract_eq) >>
+  simp[] >> gen_tac >> strip_tac >>
+  conj_tac >- (
+    match_mp_tac (UNDISCH abstract_in_funspace) >>
+    simp[boolean_in_boolset] ) >>
+  Q.ISPECL_THEN[`mem`,`in_bool`,`ina`]mp_tac (GEN_ALL range_in_fun) >>
+  discharge_hyps >- ( simp[is_in_in_bool] ) >>
+  strip_tac >> simp[range_in_bool] >>
+  Q.ISPECL_THEN[`mem`,`in_bool`,`ina`]mp_tac (GEN_ALL range_in_fun) >>
+  discharge_hyps >- ( simp[is_in_in_bool] ) >>
+  strip_tac >> simp[range_in_bool] >>
+  conj_tac >- (
+    match_mp_tac (UNDISCH abstract_in_funspace) >>
+    simp[in_bool_def,boolean_in_boolset] ) >>
+  match_mp_tac (UNDISCH abstract_eq) >>
+  simp[in_bool_def,boolean_in_boolset] >>
+  simp[boolean_def] >> rw[true_neq_false] >>
+  spose_not_then strip_assume_tac >>
+  metis_tac[is_in_finv_right])
+
+val _ = save_thms
+  ["good_context_is_in_in_bool","good_context_is_in_in_fun",
+   "good_context_lookup_bool","good_context_lookup_fun",
+   "good_context_extend_tmval","good_context_instance_equality"]
+  [ good_context_is_in_in_bool , good_context_is_in_in_fun ,
+    good_context_lookup_bool , good_context_lookup_fun ,
+    good_context_extend_tmval , good_context_instance_equality ]
 
 val _ = export_theory()
