reflectionDemoScript.sml
@@ -1,0 +1,7 @@
+open HolKernel boolLib bossLib lcsymtacs
+open reflectionLib
+val _ = new_theory"reflectionDemo"
+
+val _ = save_thm("example",prop_to_loeb_hyp``0 = 1``)
+
+val _ = export_theory()
