reflectionLib.sml
@@ -1,0 +1,160 @@
+structure reflectionLib = struct
+local
+  open HolKernel boolLib bossLib lcsymtacs listSimps stringSimps
+  open miscLib pairSyntax stringSyntax listSyntax holSyntaxSyntax
+  open reflectionTheory pred_setTheory setSpecTheory holSyntaxTheory holSyntaxExtraTheory holSemanticsTheory holSemanticsExtraTheory
+  open basicReflectionLib
+
+  val MID_EXISTS_AND_THM = prove(
+    ``(?x. P x /\ Q /\ R x) <=> (Q /\ ?x. P x /\ R x)``,
+    metis_tac[])
+  val eval = SIMP_CONV (std_ss++LIST_ss)
+    [typeof_def,codomain_def,typesem_def,
+     term_ok_def,WELLTYPED_CLAUSES,
+     type_ok_def,type_11]
+   THENC SIMP_CONV std_ss [GSYM CONJ_ASSOC,MID_EXISTS_AND_THM]
+in
+
+  val get_simpths = mapfilter (QCHANGED_CONV eval) o hyp
+  fun simp_asms th = foldl (uncurry (C simplify_assum)) th (get_simpths th)
+  val replace_asms =
+    repeat (C replace_assum good_context_is_in_in_fun) o
+    repeat (C replace_assum good_context_instance_equality) o
+    repeat (C replace_assum good_context_is_in_in_bool) o
+    repeat (C replace_assum good_context_lookup_bool) o
+    repeat (C replace_assum good_context_lookup_fun) o
+    repeat (C replace_assum TRUTH)
+  fun changed f th =
+      assert (not o curry HOLset.equal (hypset th) o hypset)
+             (f th)
+  val full_simp_asms = repeat (changed (simp_asms o replace_asms))
+
+  val in_bool_tm = ``in_bool``
+  val in_fun_tm = ``in_fun``
+
+  fun mk_in (ty : hol_type) = case type_view ty of
+      Tyapp(thy, "bool", [])        => in_bool_tm
+    | Tyapp(thy, "fun",  [ty1,ty2]) => mk_binop in_fun_tm (mk_in ty1, mk_in ty2)
+    | _                             => mk_in_var ty
+
+  fun mk_is_in_thm ty = case type_view ty of
+      Tyapp ("min","bool",[]) => good_context_is_in_in_bool
+    | Tyapp ("min","fun",[ty1,ty2]) =>
+         good_context_is_in_in_fun
+         |> ISPEC (mk_in ty1)
+         |> ISPEC (mk_in ty2)
+         |> C MATCH_MP (CONJ (mk_is_in_thm ty1)
+                             (mk_is_in_thm ty2))
+    | _ => ASSUME ``is_in ^(mk_in ty)``
+
+  fun var_to_cert v =
+    let
+      val v_deep = term_to_deep (assert is_var v)
+      val (x_deep,ty_deep) = dest_Var v_deep
+      val l = mk_comb(mk_in (type_of v),v)
+      val a = mk_eq(mk_comb(tmval,mk_pair(x_deep,ty_deep)),l)
+    in
+      MATCH_MP Var_thm (ASSUME a) |> SPEC mem
+    end
+
+  val instance_tm = Term.inst[alpha|->U]``instance``
+  fun mk_instance name ty =
+    list_mk_comb(instance_tm,[tmsig,interpretation,name,ty,tyval])
+
+  fun const_to_cert c =
+    let
+      val c_deep = term_to_deep (assert is_const c)
+      val (name_deep,ty_deep) = dest_Const c_deep
+      val l = mk_comb(mk_in (type_of c),c)
+      val a = mk_eq(mk_instance name_deep ty_deep,l)
+      val th = MATCH_MP Const_thm (ASSUME a) |> SPEC mem
+    in
+      full_simp_asms th
+    end
+
+  fun term_to_cert tm =
+    case dest_term tm of
+      VAR _ => var_to_cert tm
+    | CONST _ => const_to_cert tm
+    | COMB(t1,t2) =>
+      let
+        val c1 = term_to_cert t1
+        val c2 = term_to_cert t2
+        val (dty,rty) = dom_rng (type_of t1)
+      in
+        MATCH_MP (Comb_thm) (CONJ c1 c2)
+        |> C MATCH_MP (mk_is_in_thm dty)
+        |> C MATCH_MP (mk_is_in_thm rty)
+        |> full_simp_asms
+      end
+    | LAMB(x,b) =>
+      let
+        val (xd,tyd) = dest_Var(term_to_deep x)
+        val bd = term_to_deep b
+        val cx = var_to_cert x
+        val cb = term_to_cert b
+        val ina = cx |> concl |> lhs |> rator
+        val inb = cb |> concl |> lhs |> rator
+        val th = Abs_thm |> ISPECL[ina,inb,tm,xd,tyd,bd] |> funpow 2 UNDISCH
+        val thd = mk_is_in_thm (type_of x)
+        val thr = mk_is_in_thm (type_of b)
+        val th = MATCH_MP th thd
+        val th = MATCH_MP th thr
+        val goal = (mk_set(hyp cb @ hyp th), th |> concl |> dest_imp |> fst)
+        val th1 = TAC_PROOF(goal,
+          gen_tac >> strip_tac >>
+          SIMP_TAC bool_ss [] >>
+          match_mp_tac (MP_CANON (DISCH_ALL cb)) >>
+          ASM_SIMP_TAC (std_ss++LIST_ss++STRING_ss)
+            [combinTheory.APPLY_UPDATE_THM] >>
+          TRY (
+            conj_tac >- (
+              match_mp_tac good_context_extend_tmval >>
+              PROVE_TAC[])) >>
+          match_mp_tac EQ_SYM >>
+          match_mp_tac (MP_CANON is_in_finv_right) >>
+          PROVE_TAC[good_context_is_in_in_bool,good_context_is_in_in_fun])
+        val th2 = MP th th1
+      in
+        th2 |> UNDISCH |> full_simp_asms
+      end
+
+  fun find_equation_thms p acc =
+    let
+      val (l,r) = dest_eq p
+      val acc = find_equation_thms l acc
+      val acc = find_equation_thms r acc
+      val a = equation_def
+            |> SPECL[term_to_deep l, term_to_deep r]
+            |> SYM
+            |> SIMP_RULE (srw_ss())[]
+    in
+      a::acc
+    end handle HOL_ERR _ => acc
+
+  fun prop_to_loeb_hyp p =
+    let
+      val cert = term_to_cert p
+      val equation_intro_rule = PURE_REWRITE_RULE (find_equation_thms p [])
+      val th2 = AP_TERM``finv in_bool`` cert
+      val th3 =
+        is_in_finv_left
+        |> Q.ISPEC`in_bool`
+        |> C MATCH_MP good_context_is_in_in_bool
+        |> (fn th => CONV_RULE (LAND_CONV (REWR_CONV th)) th2)
+        |> EQ_IMP_RULE |> snd
+      val th4 = MATCH_MP finv_in_bool_True th3
+      val inst_tmsig = Q.INST[`tmsig`|->`tmsof(sigof(thyof ctxt))`]
+      val th5 = th4 |> inst_tmsig
+      val th = Q.SPEC`thyof ctxt` provable_imp_eq_true
+             |> SPECL [interpretation,valuation]
+             |> funpow 3 UNDISCH
+             |> SPEC (th5 |> concl |> rator |> rand |> lhs |> rand)
+      val th6 = MATCH_MP mp_lemma (CONJ th5 th)
+              |> equation_intro_rule
+              |> C simplify_assum (inst_tmsig (SPEC_ALL good_context_def))
+    in
+      simp_asms th6
+    end
+
+end end
